FastSubst fixes
- lots of fixes
- plus some proofs.

theories/FastSubst.v
@@ -1,7 +1,9 @@
+Require Import Coq.Lists.List.
 Require Import Coq.FSets.FMapPositive.
 Require Import Coq.PArith.BinPos.
 Require Import ExtLib.Core.RelDec.
 Require Import ExtLib.Data.Nat.
+Require Import ExtLib.Tactics.
 Require Import MirrorCore.ExprI.
 Require Import MirrorCore.Subst2.
 
@@ -15,8 +17,6 @@ Section parametric.
   Variables typ expr : Type.
   Variable typD : list Type -> typ -> Type.
   Variable Expr_expr : @Expr typ typD expr.
-
-  Variable mentionsU : expr -> uvar -> Prop.
 
   Definition pmap := t.
   Definition pset := pmap unit.
@@ -34,82 +34,372 @@ Section parametric.
                                  end) (pset_union ra rb)
     end.
 
-  Record fast_subst : Type :=
-  { subst : pmap expr
-  ; open : pmap pset
-  }.
-
-  Definition WellFormed_fast_subst (fs : fast_subst) : Prop :=
-    (forall p e,
-       find p fs.(subst) = Some e ->
-       forall u s,
-         mentionsU e (Pos.to_nat u) ->
-         find u fs.(open) = Some s ->
-         In_pset p s).
-
+  Variable mentionsU : expr -> uvar -> Prop.
   Variable get_mentions_instantiate : (uvar -> option expr) -> expr -> pset * expr.
   Variable instantiate : (uvar -> option expr) -> expr -> expr.
 
+  Definition ExprData : Type :=
+    sum (prod expr pset) pset.
+
+  Definition fast_subst : Type :=
+    pmap ExprData.
+
   Definition to_key : nat -> positive := fun x => Pos.of_nat (S x).
+  Definition from_key : positive -> nat := fun x => pred (Pos.to_nat x).
+
+  Definition mentionsOnly (e : expr) (s : pset) : Prop :=
+    forall u,
+      mentionsU e u ->
+      find (to_key u) s = Some tt.
+
+  Definition mentionedBy (k : positive) (ps : pset) (fs : fast_subst) : Prop :=
+    forall k' e m,
+      find k' fs = Some (inl (e,m)) ->
+      mentionsU e (from_key k) ->
+      find k' ps = Some tt.
+
+  Definition mentionsNone u (fs : fast_subst) : Prop :=
+    forall p' : positive,
+      match find p' fs with
+        | Some (inl (e,_)) => ~mentionsU e u
+        | _ => True
+      end.
+
+  Definition WellFormed_fast_subst (fs : fast_subst) : Prop :=
+    forall p,
+      match find p fs with
+        | Some e =>
+          match e with
+            | inl (e, m) =>
+              mentionsOnly e m /\ mentionsNone (from_key p) fs
+            | inr mb =>
+              mentionedBy p mb fs
+          end
+        | None => mentionedBy p (empty _) fs
+      end.
+
+  Theorem to_key_from_key : forall x, from_key (to_key x) = x.
+  Proof.
+    unfold to_key, from_key.
+    intros. rewrite Pnat.Nat2Pos.id. reflexivity. auto.
+  Qed.
+
+  Theorem from_key_to_key : forall x, to_key (from_key x) = x.
+  Proof.
+    unfold to_key, from_key.
+    intros.
+    remember (Pos.to_nat x). destruct n.
+    { exfalso.
+      generalize (Pnat.Pos2Nat.is_pos x). omega. }
+    { simpl pred. rewrite Heqn.
+      rewrite Pnat.Pos2Nat.id. reflexivity. }
+  Qed.
+
+  Definition fs_lookup (s : fast_subst) (u : uvar) : option expr :=
+    match find (to_key u) s with
+      | Some (inl (e,_)) => Some e
+      | _ => None
+    end.
 
   Definition fast_subst_lookup (u : uvar) (s : fast_subst) : option expr :=
-    find (to_key u) s.(subst).
+    match find (to_key u) s with
+      | Some (inl (e,_)) => Some e
+      | _ => None
+    end.
 
   Let RelDec_eq_uvar : RelDec (@eq uvar) := RelDec_eq.
   Local Existing Instance RelDec_eq_uvar.
 
+  Definition set_helper_mentionedBy (u : uvar) (up : positive) (e : expr) (mb : pset)
+             (fs : fast_subst) : option fast_subst :=
+    let (mentions, e_inst) :=
+        @get_mentions_instantiate (fs_lookup fs) e
+    in
+    if find up mentions then None
+    else
+      Some (fold (fun p _ acc =>
+                    match find p acc with
+                      | None =>
+                        acc (** dead code **)
+                      | Some (inr mb) =>
+                        acc (** dead code **)
+                      | Some (inl (e,m)) =>
+                        add p (inl (instantiate (fun x => if x ?[ eq ] u then
+                                                            Some e_inst
+                                                          else None) e,
+                                    remove up (pset_union mentions m))) acc
+                    end)
+                 mb
+                 (fold (fun p _ acc =>
+                          match find p acc with
+                            | None =>
+                              add p (inr (add up tt (empty _))) acc
+                            | Some (inr mb) =>
+                              add p (inr (add up tt mb)) acc
+                            | Some (inl (e,m)) =>
+                              (** dead code **) acc
+                          end)
+                       mentions
+                       (add up (inl (e_inst, mentions)) fs))).
+
   Definition fast_subst_set (u : uvar) (e : expr) (s : fast_subst)
   : option fast_subst :=
     let up := to_key u in
-    match @get_mentions_instantiate (fun u => find (to_key u) s.(subst)) e with
-      | (opens, e_inst) =>
-        if find up opens then None
-        else
-          Some (fold (fun p _ acc =>
-                        (** uvar p mentions u **)
-                        match find p s.(subst) with
-                          | None => (** dead code **) acc
-                          | Some e =>
-                            {| subst :=
-                                 add p (instantiate (fun x => if x ?[ eq ] u then
-                                                                Some e_inst
-                                                              else None) e) acc.(subst)
-                             ; open :=
-                                 (** TODO: this should be done with modify **)
-                                 add p match find p acc.(open) with
-                                         | None => opens
-                                         | Some opens' =>
-                                           remove up (pset_union opens opens')
-                                       end acc.(open)
-                            |}
-                        end)
-                     (match find up s.(open) with
-                        | None => empty _
-                        | Some x => x
-                      end) {| subst := add up e_inst s.(subst)
-                            ; open := add up opens s.(open) |})
+    match find up s with
+      | Some (inl _) => None
+      | Some (inr mb) => set_helper_mentionedBy u up e mb s
+      | None => set_helper_mentionedBy u up e (empty _) s
     end.
 
   Definition fast_subst_empty : fast_subst :=
-    {| subst := empty _ ; open := empty _ |}.
+    empty _.
 
   Fixpoint fast_subst_pull' (base : positive) (n : nat) (fs : fast_subst) {struct n}
-  : option (fast_subst * list expr) :=
+  : option fast_subst :=
     match n with
-      | 0 => Some (fs, nil)
+      | 0 => Some fs
       | S n =>
-        match find base fs.(subst) with
-          | None => None
-          | Some x =>
-            fast_subst_pull' (Pos.succ base) n {| subst := remove base fs.(subst)
-                                                ; open := fs.(open) |}
+        match find base fs with
+          | None
+          | Some (inr _) => None
+          | Some (inl _) =>
+            fast_subst_pull' (Pos.succ base) n (remove base fs)
         end
     end.
 
   Definition fast_subst_pull (base : uvar) := fast_subst_pull' (to_key base).
 
+  Fixpoint filter_map T U (f : T -> option U) (ls : list T) : list U :=
+    match ls with
+      | nil => nil
+      | l :: ls => match f l with
+                     | None => filter_map f ls
+                     | Some x => x :: filter_map f ls
+                   end
+    end.
+
+
   Instance Subst_fast_subst : Subst fast_subst expr :=
-    fast_subst_lookup.
+  { lookup := fast_subst_lookup
+  ; domain := fun x => filter_map (fun x =>
+                                     match snd x with
+                                       | inl _ => Some (from_key (fst x))
+                                       | _ => None
+                                     end) (elements x)
+  }.
+
+  Definition WellTyped_fast_subst (tus tvs : EnvI.tenv typ) (s : fast_subst) : Prop :=
+    forall u e, lookup u s = Some e ->
+                match List.nth_error tus u with
+                  | None => False
+                  | Some t => Safe_expr tus tvs e t
+                end.
+
+  Definition substD_fast_subst (us vs : EnvI.env typD) (s : fast_subst) : list Prop :=
+    fold (fun p e acc =>
+            match e with
+              | inl (e,_) =>
+                match List.nth_error us (from_key p) with
+                  | None => False :: acc
+                  | Some (existT ty val) =>
+                    match exprD us vs e ty with
+                      | Some val' => (val' = val) :: acc
+                      | None => False :: acc
+                    end
+                end
+              | inr _ => acc
+            end) s nil.
+
+  Definition substD_fast_subst' (us vs : EnvI.env typD) (s : fast_subst) : list Prop :=
+    List.map (fun p_e =>
+           let '(p,e) := p_e in
+           match e with
+             | inl (e,_) =>
+               match List.nth_error us (from_key p) with
+                 | None => False
+                 | Some (existT ty val) =>
+                   match exprD us vs e ty with
+                     | Some val' => (val' = val)
+                     | None => False
+                   end
+               end
+             | inr _ => True
+           end) (elements s).
+
+  Lemma Forall_cons_iff : forall T (P : T -> Prop) l ls,
+                            Forall P (l :: ls) <-> P l /\ Forall P ls.
+  Proof.
+    clear.
+    intuition;
+      inversion H; auto.
+  Qed.
+  Lemma Forall_app : forall T (P : T -> Prop) ls ls',
+                       Forall P (ls ++ ls') <-> Forall P ls /\ Forall P ls'.
+  Proof.
+    induction ls; simpl in *; intros.
+    { intuition. }
+    { do 2 rewrite Forall_cons_iff. rewrite IHls. intuition. }
+  Qed.
+
+  Theorem substD_fast_subst_substD_fast_subst'
+  : forall us vs s,
+      Forall (fun x => x) (substD_fast_subst us vs s) <->
+      Forall (fun x => x) (substD_fast_subst' us vs s).
+  Proof.
+    unfold substD_fast_subst, substD_fast_subst'; intros.
+    rewrite fold_1.
+    assert (forall l,
+                      (Forall (fun x : Prop => x)
+                              (fold_left
+                                 (fun (a : list Prop) (p : key * (expr * pset + pset)) =>
+                                    match snd p with
+                                      | inl (e, _) =>
+                                        match nth_error us (from_key (fst p)) with
+                                          | Some (existT ty val) =>
+                                            match exprD us vs e ty with
+                                              | Some val' => (val' = val) :: a
+                                              | None => False :: a
+                                            end
+                                          | None => False :: a
+                                        end
+                                      | inr _ => a
+                                    end) (elements s) l)
+                      <->
+                      Forall (fun x : Prop => x)
+                             (l ++ List.map
+                                (fun p_e : positive * (expr * pset + pset) =>
+                                   match p_e with
+                                     | (p, inl (e0, _)) =>
+                                       match nth_error us (from_key p) with
+                                         | Some (existT ty val) =>
+                                             match exprD us vs e0 ty with
+                                               | Some val' => val' = val
+                                               | None => False
+                                             end
+                                         | None => False
+                                       end
+                                     | (p, inr _) => True
+                                   end) (elements s)))
+           ).
+    { induction (elements s).
+      { simpl. intros. rewrite app_nil_r. intuition. }
+      { intros. destruct a. destruct e.
+        { simpl in *. destruct p0.
+          destruct (nth_error us (from_key p)).
+          { destruct s0. destruct (exprD us vs e x).
+            { rewrite IHl.
+              repeat rewrite Forall_app. repeat rewrite Forall_cons_iff.
+              tauto. }
+            { rewrite IHl.
+              repeat rewrite Forall_app. repeat rewrite Forall_cons_iff.
+              tauto. } }
+          { rewrite IHl.
+            repeat rewrite Forall_app. repeat rewrite Forall_cons_iff.
+            tauto. } }
+        { simpl. rewrite IHl.
+          repeat rewrite Forall_app. repeat rewrite Forall_cons_iff.
+          tauto. } } }
+    { specialize (H nil).
+      simpl in *. apply H. }
+  Qed.
+
+  Lemma WellTyped_lookup_fast_subst
+  : forall (u v : EnvI.tenv typ) (s : fast_subst) (uv : nat) (e : expr),
+      WellFormed_fast_subst s ->
+      WellTyped_fast_subst u v s ->
+      lookup uv s = Some e ->
+      exists t0 : typ, List.nth_error u uv = Some t0 /\ Safe_expr u v e t0.
+  Proof.
+    unfold WellTyped_fast_subst; simpl; intros.
+    apply H0 in H1.
+    forward. eauto.
+  Qed.
+
+  (** TODO: Move **)
+  Lemma Forall_map
+  : forall T U (f : T -> U) P ls,
+      Forall P (List.map f ls) <-> Forall (fun x => P (f x)) ls.
+  Proof.
+    induction ls; simpl.
+    { split; intros; constructor. }
+    { split; inversion 1; intros; subst; constructor; auto.
+      apply IHls. auto. apply IHls. auto. }
+  Qed.
+
+  Lemma substD_lookup_fast_subst
+  : forall (u v : EnvI.env typD) (s : fast_subst) (uv : nat) (e : expr),
+      WellFormed_fast_subst s ->
+      lookup uv s = Some e ->
+      List.Forall (fun x : Prop => x) (substD_fast_subst u v s) ->
+      exists val : sigT (typD nil),
+        List.nth_error u uv = Some val /\
+        exprD u v e (projT1 val) = Some (projT2 val).
+  Proof.
+    simpl. intros. clear H.
+    unfold fast_subst_lookup in *; simpl in *.
+    forward. inv_all; subst.
+    rewrite substD_fast_subst_substD_fast_subst' in H1.
+    unfold substD_fast_subst' in H1.
+    rewrite Forall_map in H1.
+    generalize (elements_correct s (to_key uv) H2).
+    intros.
+    eapply Forall_forall in H1; eauto.
+    simpl in *.
+    forward. subst.
+    rewrite to_key_from_key in *. eauto.
+  Qed.
+
+  Lemma in_filter_map_iff : forall T U (P : T -> option U) ls x,
+                              List.In x (filter_map P ls) <->
+                              exists y, P y = Some x /\ List.In y ls.
+  Proof.
+    clear.
+    induction ls; simpl.
+    { intuition. destruct H; intuition. }
+    { intuition.
+      { consider (P a); intros.
+        { destruct H0. subst. eauto.
+          eapply IHls in H0. destruct H0. intuition; eauto. }
+        { eapply IHls in H0. destruct H0; intuition; eauto. } }
+      { destruct H. destruct H.
+        destruct H0; subst.
+        { rewrite H. left. auto. }
+        { destruct (P a); try right; apply IHls; eauto. } } }
+  Qed.
+
+  Lemma WellFormed_domain_fast_subst
+  : forall (s : fast_subst) (ls : list nat),
+      WellFormed_fast_subst s ->
+      domain s = ls -> forall n : nat, List.In n ls <-> lookup n s <> None.
+  Proof.
+    intros; subst.
+    unfold domain, fast_subst_lookup. simpl.
+    unfold fast_subst_lookup.
+    rewrite in_filter_map_iff.
+    split; intros.
+    { destruct H0. intuition.
+      forward. inv_all; subst.
+      rewrite from_key_to_key in H1.
+      generalize (elements_complete s (fst x) (snd x)).
+      unfold ExprData in *.
+      cutrewrite ((fst x, snd x) = x); [ | (destruct x; reflexivity) ].
+      intros. apply H2 in H3. rewrite H3 in H1. rewrite H0 in *.
+      destruct p; congruence. }
+    { generalize (elements_correct s (to_key n)).
+      forward. subst.
+      specialize (H4 _ eq_refl).
+      eexists. split; eauto. simpl.
+      rewrite to_key_from_key. auto. }
+  Qed.
+
+  Instance SubstOk_fast_subst : SubstOk _ Subst_fast_subst :=
+  { WellFormed_subst := WellFormed_fast_subst
+  ; WellTyped_subst := WellTyped_fast_subst
+  ; substD := substD_fast_subst
+  ; WellTyped_lookup := WellTyped_lookup_fast_subst
+  ; substD_lookup := substD_lookup_fast_subst
+  ; WellFormed_domain := WellFormed_domain_fast_subst
+  }.
 
   Instance SubstUpdate_fast_subst : SubstUpdate fast_subst expr :=
   { empty := fast_subst_empty
@@ -117,22 +407,98 @@ Section parametric.
   ; set := fast_subst_set
   }.
 
-(**
-    let zs :=  in
-    let opens := fold (fun p _ acc =>
-                         match find p s.(open) with
-                           | None => acc
-                           | Some acc' => pset_join acc acc'
-                         end) (get_mentions e) pset_empty in
-**)
+  Hypothesis get_mentions_instantiateOk
+  : forall f e s e',
+      get_mentions_instantiate f e = (s, e') ->
+      e' = instantiate f e /\
+      (forall u, mentionsU e u -> mem (to_key u) s = true).
+
+  Definition self_instantiated (f : uvar -> option expr) : Prop :=
+    forall x e, f x = Some e ->
+                forall y,
+                  f y <> None -> ~mentionsU e y.
+
+  Hypothesis mentionsU_instantiate_complete
+  : forall f, self_instantiated f ->
+              forall u e,
+                mentionsU (instantiate f e) u ->
+                f u = None.
+  Hypothesis instantiate_exprD
+  : forall f us vs e t,
+      (forall u t' val,
+         f u = Some e ->
+         nth_error us u = Some (existT _ t' val) /\
+         exprD us vs e t' = Some val) ->
+      exprD us vs (instantiate f e) t = exprD us vs e t.
+  Hypothesis instantiate_typed
+  : forall f tus tvs e t,
+      (forall u t',
+         f u = Some e ->
+         nth_error tus u = Some t' /\
+         Safe_expr tus tvs e t') ->
+      Safe_expr tus tvs (instantiate f e) t <-> Safe_expr tus tvs e t.
+
+  Lemma All_set_fast_subst
+  : forall (uv : nat) (e : expr) (s s' : fast_subst),
+      WellFormed_subst s ->
+      set uv e s = Some s' ->
+      WellFormed_subst s' /\
+      forall tus tvs t,
+        WellTyped_subst tus tvs s ->
+        Safe_expr tus tvs e t ->
+        nth_error tus uv = Some t ->
+        WellTyped_subst tus tvs s' /\
+        forall us vs,
+          Forall (fun x => x) (substD us vs s') ->
+          Forall (fun x => x) (substD us vs s) /\
+          (forall tv : sigT (typD nil),
+             nth_error us uv = Some tv -> exprD us vs e (projT1 tv) = Some (projT2 tv)).
+  Proof.
+    simpl. unfold fast_subst_set; simpl; intros.
+    forward. inv_all.
+    match goal with
+      | |- ?G =>
+        assert (forall mb, mentionedBy (to_key uv) mb s ->
+                           set_helper_mentionedBy uv (to_key uv) e mb s = Some s' ->
+                           G)
+    end.
+    { admit. }
+    { red in H. specialize (H (to_key uv)).
+      destruct (find (to_key uv) s); eauto.
+      { destruct e0; try congruence; eauto. } }
+  Qed.
+
+  Instance SubstUpdateOk_fast_subst : SubstUpdateOk SubstUpdate_fast_subst _.
+  Proof.
+    constructor.
+    { red; simpl. red. unfold fast_subst_empty. simpl.
+      intros. rewrite gempty. red. intros.
+      rewrite gempty in H. congruence. }
+    { compute. constructor. }
+    { red. simpl. red. simpl.
+      unfold fast_subst_lookup.
+      intros. destruct (to_key u0); compute in H; try congruence. }
+    { intros.
+      specialize (@All_set_fast_subst uv e s s' H H0).
+      tauto. }
+    { intros.
+      destruct (@All_set_fast_subst uv e s s' H H3).
+      specialize (@H5 u v t0 H0 H2 H1).
+      tauto. }
+    { admit. }
+    { admit. }
+    { admit. }
+    { admit. }
+  Qed.
+
 End parametric.
 
-(** For Expr **)
+(** For Expr (TODO: this should move to Ext/ExprSubst **)
 Section funced.
   Require Import MirrorCore.Ext.ExprCore.
   Require Import MirrorCore.Ext.ExprSubst.
 
-  Variable func : Type.
+  Let func : Type := nat.
 
   Definition instantiate : (uvar -> option (expr func)) -> expr func -> expr func :=
     fun z => ExprSubst.instantiate z 0.
@@ -143,7 +509,7 @@ Section funced.
       | Inj _ => acc
       | App l r => get_mentions l (get_mentions r acc)
       | Abs _ e => get_mentions e acc
-      | UVar u => PositiveMap.add (Pos.of_nat (S u)) tt acc
+      | UVar u => PositiveMap.add (to_key u) tt acc
     end.
 
   Definition get_mentions_instantiate (i : uvar -> option (expr func)) (e : expr func)
@@ -151,17 +517,18 @@ Section funced.
     let e' := instantiate i e in
     (get_mentions e' (PositiveMap.empty _), e').
 
-(*
   Definition l := @fast_subst_lookup (expr func).
   Definition e := @fast_subst_empty (expr func).
   Definition s := @fast_subst_set (expr func) get_mentions_instantiate instantiate.
-
-  Check s.
+  Definition d := @fast_subst_pull (expr func).
 
   Require Import ExtLib.Structures.Monad.
   Require Import ExtLib.Data.Monads.OptionMonad.
 
-  Eval compute in bind (s 0 (Inj 0) e) (l 0).
-*)
+  Check d.
+
+  Eval compute in s 0 (UVar 1) e.
+  Eval compute in bind (s 1 (Inj 2) e) (fun x => bind (s 0 (UVar 1) x) (d 1 1)).
+  Eval compute in bind (s 0 (UVar 1) e) (fun x => bind (s 1 (Inj 2) x) (d 0 2)).
 
 End funced.
